@prefix dc: <http://purl.org/dc/elements/1.1/> .
@prefix dcat: <http://www.w3.org/ns/dcat#> .
@prefix dct: <http://purl.org/dc/terms/> .
@prefix euvoc: <http://publications.europa.eu/ontology/euvoc#> .
@prefix foaf: <http://xmlns.com/foaf/0.1/> .
@prefix lcp: <https://www.ieawindtask43.org/ontoforge/life-cycle-phase-din-spec-91303/> .
@prefix org: <http://www.w3.org/ns/org#> .
@prefix owl: <http://www.w3.org/2002/07/owl#> .
@prefix prov: <http://www.w3.org/ns/prov#> .
@prefix qb: <http://purl.org/linked-data/cube#> .
@prefix rdf: <http://www.w3.org/1999/02/22-rdf-syntax-ns#> .
@prefix rdfs: <http://www.w3.org/2000/01/rdf-schema#> .
@prefix schema: <http://schema.org/> .
@prefix sh: <http://www.w3.org/ns/shacl#> .
@prefix skos: <http://www.w3.org/2004/02/skos/core#> .
@prefix skosthes: <http://purl.org/iso25964/skos-thes#> .
@prefix skosxl: <http://www.w3.org/2008/05/skos-xl#> .
@prefix wpl: <https://www.ieawindtask43.org/ontoforge/life-cycle-phase-process-taxonomy/> .
@prefix xsd: <http://www.w3.org/2001/XMLSchema#> .

<https://www.ieawindtask43.org/ontoforge/life-cycle-phase-din-spec-91303/> a skos:ConceptScheme;
  dct:creator "Deutsche Institut für Normung e. V."@en;
  dct:description "SKOS Taxonomy of life-cycle phases according to DIN SPEC 91303"@en;
  dct:license <http://creativecommons.org/licenses/by/4.0/>;
  dct:title "Life Cycle Phase Specification DIN SPEC 91303"@en;
  owl:versionInfo "0.0.1"@en;
  skos:hasTopConcept lcp:LifeCyclePhase;
  skos:prefLabel "LCP-DIN-91303"@en .

lcp:LifeCyclePhase a skos:Concept;
  skos:inScheme <https://www.ieawindtask43.org/ontoforge/life-cycle-phase-din-spec-91303/>;
  skos:narrower lcp:Decommissioning, lcp:Preparation, lcp:Usage;
  skos:prefLabel "Life Cycle Phase"@en;
  skos:topConceptOf <https://www.ieawindtask43.org/ontoforge/life-cycle-phase-din-spec-91303/> .

lcp:Preparation a skos:Concept;
  skos:broader lcp:LifeCyclePhase;
  skos:inScheme <https://www.ieawindtask43.org/ontoforge/life-cycle-phase-din-spec-91303/>;
  skos:narrower lcp:Commissioning, lcp:Construction, lcp:Design, lcp:Planning, lcp:PurchaseDivFabrication;
  skos:prefLabel "Preparation"@en, "Vorbereitung"@de .

lcp:Planning a skos:Concept;
  skos:broader lcp:Preparation;
  skos:definition """Conception of wind turbine.
Site selection, wind study, nature conservation, purchase / lease of ground."""@en,
    """Konzipierung WEA.
Standortauswahl, Windgutachten, Flora-Fauna-Schutz, Sicherung des Grundstück."""@de;
  skos:inScheme <https://www.ieawindtask43.org/ontoforge/life-cycle-phase-din-spec-91303/>;
  skos:prefLabel "Planning"@en, "Planung"@de .

lcp:Design a skos:Concept;
  skos:broader lcp:Preparation;
  skos:definition """Detailauslegung WEA inkl. Prototyp und Test bis zur Zertifizierung.
Engineering Windpark bis zur Baugenehmigung."""@de,
    """Detailed design of wind turbine including prototyping, test and certification.
Development of power plant until permission."""@en;
  skos:inScheme <https://www.ieawindtask43.org/ontoforge/life-cycle-phase-din-spec-91303/>;
  skos:prefLabel "Design"@en, "Konstruktion"@de .

lcp:PurchaseDivFabrication a skos:Concept;
  skos:broader lcp:Preparation;
  skos:definition """Fertigung und Überwachung, Einkauf aller Komponenten, Zusammenbau der Sub-Systeme zur Auslieferung.
Kaufverträge, Vertrag Netzanbindung, Versicherungen."""@de,
    """Manufacturing and supervision, purchase of components, assembly of sub-systems, delivery.
Purchase contract, contract for grid connection, insurance."""@en;
  skos:inScheme <https://www.ieawindtask43.org/ontoforge/life-cycle-phase-din-spec-91303/>;
  skos:prefLabel "Beschaffung / Fertigung"@de, "Purchase / Fabrication"@en .

lcp:Construction a skos:Concept;
  skos:broader lcp:Preparation;
  skos:definition "Transport, Errichtung der WEA und der Infrastruktur, Bauüberwachung"@de,
    "Transportation, erection of wind turbines, construction of infrastructure, supervision."@en;
  skos:inScheme <https://www.ieawindtask43.org/ontoforge/life-cycle-phase-din-spec-91303/>;
  skos:prefLabel "Construction"@en, "Errichtung"@de .

lcp:Commissioning a skos:Concept;
  skos:broader lcp:Preparation;
  skos:definition "Commissioning of wind turbines and infrastructur including test run and proof / acceptance by the grid operators as well as by authorities"@en,
    "Inbetriebsetzung der WEA und der Infrastruktur inkl. Probebetrieb und Prüfung bzw. Abnahme durch den WEA-, Netz-Betreiber und Genehmigungsbehörde"@de;
  skos:inScheme <https://www.ieawindtask43.org/ontoforge/life-cycle-phase-din-spec-91303/>;
  skos:prefLabel "Commissioning"@en, "Inbetriebnahme"@de .

lcp:Usage a skos:Concept;
  skos:broader lcp:LifeCyclePhase;
  skos:inScheme <https://www.ieawindtask43.org/ontoforge/life-cycle-phase-din-spec-91303/>;
  skos:narrower lcp:Maintenance, lcp:ProductionDivOperation, lcp:Shutdown;
  skos:prefLabel "Nutzung"@de, "Usage"@en .

lcp:ProductionDivOperation a skos:Concept;
  skos:broader lcp:Usage;
  skos:definition """Einsatzplanung;
Überwachung (Nachweisprüfung);
Performanceanalyse;
Reporting;
Verträge/Pflichten;
Stromhandel;
Versicherungen
Beschaffung (Dienstleistungen, Ersatz,…);
Anlagenverantwortung;
IH-Strategie"""@de,
    """Life-cylce phase which includes the following activities: 
Operational planning;
Regular surveying;
Performance analysis;
Reporting;
Contracts / obligations;
Trading of electricity;
Insurances;
Purchase of consultancies;
Responsability for the facilities;
O&M strategy"""@en;
  skos:inScheme <https://www.ieawindtask43.org/ontoforge/life-cycle-phase-din-spec-91303/>;
  skos:prefLabel "Production / Operation"@en, "Produktion / Betrieb"@de .

lcp:Maintenance a skos:Concept;
  skos:broader lcp:Usage;
  skos:definition "Regular service, maintenance, improvements."@en, """Wartung
Inspektion
Instandsetzung
Verbesserung"""@de;
  skos:inScheme <https://www.ieawindtask43.org/ontoforge/life-cycle-phase-din-spec-91303/>;
  skos:prefLabel "Instandhaltung"@de, "Maintenance"@en .

lcp:Shutdown a skos:Concept;
  skos:broader lcp:Usage;
  skos:definition "Shutdown due to limited permission or technical defects or planned decommissioning."@en,
    "Stilllegung aufgrund rechtlicher Vorgaben, technischer Mängel oder bevorstehendem Rückbau"@de;
  skos:inScheme <https://www.ieawindtask43.org/ontoforge/life-cycle-phase-din-spec-91303/>;
  skos:prefLabel "Shutdown"@en, "Stilllegung"@de .

lcp:Decommissioning a skos:Concept;
  skos:broader lcp:LifeCyclePhase;
  skos:exactMatch wpl:8Decomissioning;
  skos:inScheme <https://www.ieawindtask43.org/ontoforge/life-cycle-phase-din-spec-91303/>;
  skos:narrower lcp:Dismantling, lcp:Planningofdismantling;
  skos:prefLabel "Decommissioning"@en, "Rückabwicklung"@de .

lcp:Planningofdismantling a skos:Concept;
  skos:broader lcp:Decommissioning;
  skos:definition "Preparation of dismantling, purchase of components."@en, "Vorbereitung des Rückbaus"@de;
  skos:inScheme <https://www.ieawindtask43.org/ontoforge/life-cycle-phase-din-spec-91303/>;
  skos:prefLabel "Planning of dismantling"@en, "Rückbau-Planung"@de .

lcp:Dismantling a skos:Concept;
  skos:broader lcp:Decommissioning;
  skos:definition "Abbau, Wiederverwertung, Entsorgung"@de, "Dismantling, recycling, disposal"@en;
  skos:inScheme <https://www.ieawindtask43.org/ontoforge/life-cycle-phase-din-spec-91303/>;
  skos:prefLabel "Dismantling"@en, "Rückbau"@de .
